more buffer refinements

Is0/Basic.lean
@@ -66,33 +66,35 @@ end Map
 end Map
 
 abbrev Buffer (α : Type) := List (List α)
-
 def Back := ℕ
 
 @[simp]
 def Back.toNat (back : Back) : ℕ := back
 
 instance : HSub ℕ Back Back := ⟨λ lhs rhs => lhs - rhs.toNat⟩
-
 instance : OfNat Back n := ⟨n⟩
-instance {α : Type}: GetElem (Buffer α) (Back × ℕ) α λ buf i =>
-                       ∃ (h : i.1.toNat < buf.length), i.2 < (buf[i.1.toNat]'h).length :=
+
+instance {α : Type} : GetElem (Buffer α) (Back × ℕ) α λ buf i =>
+                        ∃ (h : i.1.toNat < buf.length), i.2 < (buf[i.1.toNat]'h).length :=
   ⟨λ buf i h => (buf[i.1.toNat]'h.1)[i.2]'h.2⟩
+  
+def Buffer.set {α : Type} (buf : Buffer α) (cycle : ℕ) (offset : ℕ) (val : α) : Buffer α :=
+  List.set buf cycle (buf[cycle]!.set offset val)
 
-def Buffer.get! {α} [Inhabited α] (buffer : Buffer α) (offset : ℕ) (back : Back := 0) : α :=
-  buffer[(back, offset)]!
+inductive VarType := | FeltTag | PropTag | ListFeltTag
+open VarType
 
-def Buffer.set (buffer : Buffer α) (offset : ℕ) (currentCycle : ℕ) : Buffer α := 
-  buffer[
+structure Variable (tag : VarType) :=
+  name : String
 
 -- The first three fields map variable names to values. The last is an
 -- append-only stack of the expressions we assert are equal to zero via `Eqz`.
 structure State where
-  felts : Map String Felt
-  props : Map String Prop
-  buffers : Map String (Buffer Felt)
+  felts       : Map String Felt
+  props       : Map String Prop
+  buffers     : Map String (Buffer Felt)
   constraints : List Prop
-  cycle : ℕ
+  cycle       : ℕ
 
 def State.update (state : State) (name : String) (x : Lit) : State :=
   match x with
@@ -119,11 +121,6 @@ lemma State.if_constraints {state₁ state₂ : State} {x : Felt} :
 
 notation:61 st "[" n:61 "]" " := " x:49 => State.update st n x
 
-inductive VarType := | FeltTag | PropTag | ListFeltTag
-
-structure Variable (tag : VarType) :=
-  name : String
-
 inductive IsNondet :=
   | InNondet
   | NotInNondet
@@ -141,20 +138,20 @@ open VarType in
 inductive Op : IsNondet → Type where
   -- Constants
   | Const : Felt → Op x
-  | True : Op x
+  | True  : Op x
   -- Arith
   | Add : Variable FeltTag → Variable FeltTag → Op x
   | Sub : Variable FeltTag → Variable FeltTag → Op x
-  | Neg : Variable FeltTag → Op x
+  | Neg : Variable FeltTag                    → Op x
   | Mul : Variable FeltTag → Variable FeltTag → Op x
-  | Pow : Variable FeltTag → ℕ → Op x
+  | Pow : Variable FeltTag → ℕ                → Op x
   -- Logic
   | Isz : Variable FeltTag → Op InNondet
   | Inv : Variable FeltTag → Op InNondet
   -- Constraints
-  | AndEqz : Variable PropTag → Variable FeltTag → Op x
+  | AndEqz  : Variable PropTag → Variable FeltTag                    → Op x
   | AndCond : Variable PropTag → Variable FeltTag → Variable PropTag → Op x
-  -- Buffers
+  -- State
   | GetBuffer : Variable ListFeltTag → Back → ℕ → Op x
 
 open Op VarType
@@ -174,40 +171,48 @@ instance : HPow (Variable FeltTag) ℕ (Op IsNondet.NotInNondet) := ⟨Op.Pow⟩
 -- Notation for Ops.
 namespace MLIRNotation
 
-scoped prefix:max "C" => Op.Const
-scoped notation:max "⊤" => Op.True
-scoped notation:max "input[" n "]" => Op.GetInput n 0
-scoped notation:max "output[" n "]" => Op.GetOutput n 0
-scoped infix:55 " &₀ " => Op.AndEqz
-scoped notation:55 " guard " c " & " x " with " y:55 => Op.AndCond x c y
-scoped prefix:57 "??₀" => Op.Isz
-scoped prefix:max "Inv" => Op.Inv
+scoped prefix  :max "C"                               => Op.Const
+scoped notation:max "⊤"                               => Op.True
+scoped notation:max "input[" n "]"                    => Op.GetInput n 0
+scoped notation:max "output[" n "]"                   => Op.GetOutput n 0
+scoped infix   :55  " &₀ "                            => Op.AndEqz
+scoped notation:55  " guard " c " & " x " with " y:55 => Op.AndCond x c y
+scoped prefix  :57  "??₀"                             => Op.Isz
+scoped prefix  :max "Inv"                             => Op.Inv
 
 end MLIRNotation
 
 instance : Inhabited Felt := ⟨-42⟩
 
--- Evaluate a pure functional circuit operation to get some kind of literal.
+def State.get! (st : State) (buf : Variable ListFeltTag) (back : Back) (offset : ℕ) : Felt := 
+  (st.buffers buf.name).get![(st.cycle - back, offset)]!
+
+-- Evaluate a pure functional circuit.
 def Op.eval {x} (st : State) (op : Op x) : Lit :=
   match op with
-  | Const x       => .Val x
-  | True          => .Constraint _root_.True
-  | GetBuffer buf back offset => .Val <| (st.buffers buf.name).get![(st.cycle - back, offset)]!
-  | Add x y       => .Val <| (st.felts x.name).get! + (st.felts y.name).get!
-  | Sub x y       => .Val <| (st.felts x.name).get! - (st.felts y.name).get!
-  | Mul x y       => .Val <| (st.felts x.name).get! * (st.felts y.name).get!
-  | Pow x y       => .Val <| (st.felts x.name).get! ^ y
-  | Neg x         => .Val <| 0 - (st.felts x.name).get!
-  | AndEqz c x    => .Constraint <| (st.props c.name).get! ∧ (st.felts x.name).get! = 0
-  | AndCond old cond inner =>
-      .Constraint <| (st.props old.name).get! ∧
-                     if (st.felts cond.name).get! = 0
-                       then _root_.True
-                       else (st.props inner.name).get!
-  | Isz x         => .Val $ if (st.felts x.name).get! = 0 then 1 else 0
-  | Inv x         => .Val $ match st.felts x.name with
-                              | some x => if x = 0 then 0 else x⁻¹
-                              | _      => default
+    -- Constants
+    | Const const => .Val const
+    | True        => .Constraint _root_.True
+    -- Arith
+    | Add lhs rhs => .Val <| (st.felts lhs.name).get! + (st.felts rhs.name).get!
+    | Sub lhs rhs => .Val <| (st.felts lhs.name).get! - (st.felts rhs.name).get!
+    | Neg lhs     => .Val <| 0                        - (st.felts lhs.name).get!
+    | Mul lhs rhs => .Val <| (st.felts lhs.name).get! * (st.felts rhs.name).get!
+    | Pow lhs rhs => .Val <| (st.felts lhs.name).get! ^ rhs
+    -- Logic
+    | Isz x => .Val <| if (st.felts x.name).get! = 0 then 1 else 0
+    | Inv x => .Val <| match st.felts x.name with
+                         | some x => if x = 0 then 0 else x⁻¹
+                         | _      => default
+    -- Constraints
+    | AndEqz c val           => .Constraint <| (st.props c.name).get! ∧ (st.felts val.name).get! = 0
+    | AndCond old cond inner =>
+        .Constraint <| (st.props old.name).get! ∧
+                       if (st.felts cond.name).get! = 0
+                         then _root_.True
+                         else (st.props inner.name).get!
+    -- State
+    | GetBuffer buf back offset => .Val <| st.get! buf back offset
 
 notation:61 "Γ " st:max " ⟦" p:49 "⟧ₑ" => Op.eval st p
 
@@ -216,6 +221,8 @@ namespace MLIRNotation
 end MLIRNotation
 
 namespace Op
+
+-- TODO(move this out)
 
 section Op
 
@@ -264,22 +271,22 @@ end Op
 end Op
 
 inductive MLIR : IsNondet → Type where
-  | Assign : String → Op x → MLIR x
-  | Eqz : Variable FeltTag → MLIR x
-  | If : Variable FeltTag → MLIR x → MLIR x
-  | Nondet : MLIR InNondet → MLIR NotInNondet
-  | Sequence : MLIR x → MLIR x → MLIR x
-  | SetOutput : ℕ → Variable FeltTag → MLIR InNondet
+  | Assign    : String               → Op x   → MLIR x
+  | Eqz       : Variable FeltTag              → MLIR x
+  | If        : Variable FeltTag     → MLIR x → MLIR x
+  | Nondet    : MLIR InNondet                 → MLIR NotInNondet
+  | Sequence  : MLIR x               → MLIR x → MLIR x
+  | Set       : Variable ListFeltTag → ℕ      → Variable FeltTag → MLIR InNondet
 
 -- Notation for MLIR programs.  
 namespace MLIRNotation
 
-scoped infix:51 "←ₐ " => MLIR.Assign
-scoped prefix:52 "?₀" => MLIR.Eqz
-scoped notation:51 "guard " c " then " x:51 => MLIR.If c x
-scoped prefix:max "nondet" => MLIR.Nondet
-scoped infixr:50 "; " => MLIR.Sequence
-scoped notation:51 (priority := high) "output[" v:51 "]" " ←ᵢ " x:51 => MLIR.SetOutput v x
+scoped infix   :51                    "←ₐ "                      => MLIR.Assign
+scoped prefix  :52                    "?₀"                       => MLIR.Eqz
+scoped notation:51                    "guard " c " then " x:51   => MLIR.If c x
+scoped prefix  :max                   "nondet"                   => MLIR.Nondet
+scoped infixr  :50                    "; "                       => MLIR.Sequence
+scoped notation:51 (priority := high) b "[" v:51 "]" " ←ᵢ " x:51 => MLIR.Set b v x
 
 end MLIRNotation
 
@@ -290,6 +297,10 @@ abbrev withEqZero (x : Felt) (st : State) : State :=
 
 @[simp]
 lemma withEqZero_def : withEqZero x st = {st with constraints := (x = 0) :: st.constraints} := rfl
+
+def State.set (st : State) (buffer : Variable ListFeltTag) (offset : ℕ) (val : Felt) : State := 
+  {st with buffers :=
+     st.buffers[buffer.name] := ((st.buffers buffer.name).get!.set offset st.cycle val)}
 
 -- Step through the entirety of a `MLIR` MLIR program from initial state
 -- `state`, yielding the post-execution state and possibly a constraint
@@ -303,15 +314,14 @@ def MLIR.run {α : IsNondet} (program : MLIR α) (st : State) : State :=
           | _       => st
     | If x program =>
         match st.felts x.name with
-          | some x => if x = 0 then st else program.run st
-          | _      => st
+          | .some x => if x = 0 then st else program.run st
+          | _       => st
     | Nondet block => block.run st
     | Sequence a b => b.run (a.run st)
-    | SetOutput i x =>
-        match st.felts x.name with
-          | .some x => 
-                       {st with buffers := st.buffers.update "output" ((st.buffers "output").get![st.cycle]!.set i x)}
-          | _       => st
+    | Set buf offset val =>
+        match st.felts val.name with
+          | .some val => st.set buf offset val
+          | _         => st
 
 @[simp]
 abbrev MLIR.runProgram (program : MLIRProgram) := program.run
