Is0/Lemmas.lean
@@ -15,27 +15,30 @@ variable {α : IsNondet} {st : State} {name : String}
 open MLIRNotation IsNondet
 open Risc0.VarType
 
--- MLIR.run def lemmas
-lemma MLIR.run_ass_def : Γ st ⟦name ←ₐ op⟧ = st[name] := Γ st ⟦op⟧ₑ := rfl
+namespace MLIR
 
-lemma MLIR.run_set_def : Γ st ⟦output[i] ←ᵢ x⟧ = 
-  match st.felts x.name with
-    | .some x => {st with output := st.output.set i x}
-    | _       => st := rfl
+lemma run_ass_def : Γ st ⟦name ←ₐ op⟧ = st[name] := Γ st ⟦op⟧ₑ := rfl
 
-lemma MLIR.run_seq_def : Γ st ⟦p₁; p₂⟧ = Γ (Γ st ⟦p₁⟧) ⟦p₂⟧ := rfl
+lemma run_set_def : Γ st ⟦buf[offset] ←ᵢ val⟧ = 
+  match st.felts val.name with
+    | .some val => st.set buf offset val
+    | _         => st := rfl
 
-lemma MLIR.run_nondet : Γ st ⟦nondet block⟧ = Γ st ⟦block⟧ := rfl
+lemma run_seq_def : Γ st ⟦p₁; p₂⟧ = Γ (Γ st ⟦p₁⟧) ⟦p₂⟧ := rfl
 
-lemma MLIR.run_set (x : Felt) (h₁ : st.felts nameₓ = some x) :
-  Γ st ⟦output[i] ←ᵢ ⟨nameₓ⟩⟧ = { st with output := st.output.set i x } := by simp [run_set_def, h₁]
+lemma run_nondet : Γ st ⟦nondet block⟧ = Γ st ⟦block⟧ := rfl
 
-lemma MLIR.run_if (x : Felt) (h₁ : st.felts name = some x) :
+lemma run_set_output (x : Felt) (h₁ : st.felts nameₓ = some x) :
+  Γ st ⟦⟨"output"⟩[i] ←ᵢ ⟨nameₓ⟩⟧ = { st with output := st.output.set i x } := by simp [run_set_def, h₁]
+
+lemma run_if (x : Felt) (h₁ : st.felts name = some x) :
   Γ st ⟦guard ⟨name⟩ then branch⟧
   = if x = 0 then st else Γ st ⟦branch⟧ := by simp [run, h₁]
 
-lemma MLIR.run_eqz (x : Felt) (h₁ : st.felts name = some x) :
+lemma run_eqz (x : Felt) (h₁ : st.felts name = some x) :
   Γ st ⟦@MLIR.Eqz α ⟨name⟩⟧ = withEqZero x st := by simp [run, h₁]
+
+end MLIR
 
 end WithMLIR 
 
